Another version of find even numbers and some cleanups

MBPP/016 FindEvenNumbers Array v1.dfy
@@ -8,25 +8,115 @@ predicate IsEven(n: int)
 }
 
 method FindEvenNumbers(arr: array<int>) returns (evenNumbers: array<int>)
-    // All numbers in the output are even and exist in the input 
-    ensures forall i :: 0 <= i < evenNumbers.Length ==> IsEven(evenNumbers[i]) && evenNumbers[i] in arr[..]
     // All even numbers in the input are in the output
-    ensures forall i :: 0 <= i < arr.Length && IsEven(arr[i]) ==> arr[i] in evenNumbers[..]
+    ensures forall x :: x in arr[..] && IsEven(x) ==> x in evenNumbers[..];
+    // If a number is not in the input, it's also not in the output 
+    ensures forall x :: x !in arr[..] ==> x !in evenNumbers[..]
+    // Relative order of even numbers is preserved
+    ensures evenNumbers[..] == filter(arr[..], IsEven)
 {
-    var evenList: seq<int> := [];
-    for i := 0 to arr.Length
-        invariant 0 <= i <= arr.Length
-        invariant 0 <= |evenList| <= i
-        invariant forall k :: 0 <= k < i && IsEven(arr[k]) ==> arr[k] in evenList
-        invariant forall k :: 0 <= k < |evenList| ==> IsEven(evenList[k]) && evenList[k] in arr[..i]
-    {
-        if IsEven(arr[i])
-        {
-            evenList := evenList + [arr[i]];
-        }
-    }
-
+    var evenList: seq<int> := filter(arr[..], IsEven);
     evenNumbers := new int[|evenList|](i requires 0 <= i < |evenList| => evenList[i]);
     assert evenList == evenNumbers[..];
+}
+
+function filter<T>(s: seq<T>, p: T -> bool) : seq<T>
+    ensures forall x :: x !in s ==> x !in filter(s, p)
+    ensures forall x :: x in s && p(x) ==> x in filter(s, p)
+    ensures |s| > 0 && p(s[0]) <==> |s| > 0  && filter(s, p) == [s[0]] + filter(s[1..], p)
+{
+    if s == [] then []
+    else 
+        if p(s[0]) then 
+            [s[0]] + filter(s[1..], p)
+        else filter(s[1..], p)
+}
+
+
+method m1() {
+//    EquivalenceLemma([1, 2, 3, 4, 5], [4, 2], IsEven);
+    var s := [1, 2, 3, 4, 5];
+    SameSequenceLemma(s, filter(s, IsEven), 4, IsEven);
+    SameSequenceLemma(s, [2, 4], 4, IsEven);
+//    assert filter([1, 2, 3, 4, 5], IsEven) == [4, 2];
+}
+
+/*
+// Prove that both seqs are equivalent
+lemma EquivalenceLemma<T>(original: seq<T>, filtered: seq<T>, p: T -> bool)
+    requires forall x :: x !in original ==> x !in filter(original, p)
+    requires forall x :: x in original && p(x) ==> x in filter(original, p)
+//    requires |original| > 0 && p(original[0]) <==> |original| > 0  && filter(original, p) == [original[0]] + filter(original[1..], p)
+    ensures filtered == filter(original, p)
+{
+    
+    if original == [] {
+        assert [] == filter(original, p);
+        if filtered == [] {
+            assert filtered == filter(original, p);
+        }
+        else {
+            // Impossible
+            assume exists k :: 0 <= k < |filtered| && filtered[k] in original;
+            assert false;
+        }
+    }
+    else {
+        if p(original[0]) {
+            assert original == [original[0]] + original[1..];
+            assert filter(original, p) == [original[0]] + filter(original[1..], p);
+            if filtered == [] {
+                // Impossible
+                assume exists k :: 0 <= k < |filtered| && filtered[k] in original;
+                assert false;
+            }
+            else {
+                assert original[0] == filtered[0]; // !!! Can't prove this
+                EquivalenceLemma(original[1..], filtered[1..], p);
+                assert filtered[1..] == filter(original[1..], p);
+                assert filtered == [original[0]] + filtered[1..];
+            }
+        }
+        else {
+            assert original == [original[0]] + original[1..];
+            assert filter(original, p) == filter(original[1..], p);
+            EquivalenceLemma(original[1..], filtered, p);
+            assert filtered == filtered;
+            assert filtered == filter(original, p);
+        }
+    }
+}
+*/
+
+// Prove that adding one element to both seqs preserves the relative order of the elements
+lemma SameSequenceLemma<T>(original: seq<T>, filtered: seq<T>, i: T, p: T -> bool) 
+    requires filtered == filter(original, p)
+    ensures p(i) ==> filtered + [i] == filter(original + [i], p)
+    ensures !p(i) ==> filtered == filter(original + [i], p)
+{
+    if original == [] {
+        assert original + [i] == [i];
+        assert filtered + [i] == [i];
+        assert p(i) ==> filter(original + [i], p) == [i];
+        assert !p(i) ==> filter(original + [i], p) == [];
+    } else {
+    if p(original[0]) {
+        assert original + [i] == [original[0]] + (original[1..] + [i]);
+        assert filter(original + [i], p) == [original[0]] + filter(original[1..] + [i], p);
+        SameSequenceLemma(original[1..], filtered[1..], i, p);
+        assert p(i) ==> filtered[1..] + [i] == filter(original[1..] + [i], p);
+        assert !p(i) ==> filtered[1..] == filter(original[1..] + [i], p);
+        assert filtered + [i] == [original[0]] + (filtered[1..] + [i]);
+        assert p(i) ==> filtered + [i] == filter(original + [i], p);
+        assert !p(i) ==> filtered == filter(original + [i], p);
+    } else {
+        assert original + [i] == [original[0]] + (original[1..] + [i]);
+        assert filter(original + [i], p) == filter(original[1..] + [i], p);
+        SameSequenceLemma(original[1..], filtered, i, p);
+        assert filtered + [i] == filtered + [i];
+        assert p(i) ==> filtered + [i] == filter(original + [i], p);
+        assert !p(i) ==> filtered == filter(original + [i], p);
+    }
+    }
 }
 
