MBPP/016 FindEvenNumbers Array v2.dfy
@@ -1,0 +1,32 @@
+/**
+ * Find even numbers from an array of numbers
+ **/
+
+predicate IsEven(n: int)
+{
+    n % 2 == 0
+}
+
+method FindEvenNumbers(arr: array<int>) returns (evenNumbers: array<int>)
+    // All even numbers in the input are in the output
+    ensures forall x :: x in arr[..] && IsEven(x) ==> x in evenNumbers[..];
+    // If a number is not in the input, it's also not in the output 
+    ensures forall x :: x !in arr[..] ==> x !in evenNumbers[..]
+    // Relative order of even numbers is preserved
+{
+    var evenList: seq<int> := [];
+    for i := 0 to arr.Length
+        invariant 0 <= i <= arr.Length
+        invariant 0 <= |evenList| <= i
+        invariant forall x :: x in arr[..i] && IsEven(x) ==> x in evenList[..]
+        invariant forall x :: x !in arr[..i] ==> x !in evenList
+    {
+        if IsEven(arr[i])
+        {
+            evenList := evenList + [arr[i]];
+        }
+    }
+
+    evenNumbers := new int[|evenList|](i requires 0 <= i < |evenList| => evenList[i]);
+    assert evenList == evenNumbers[..];
+}
